got rid of most params; must change assembly to us search for instruction directly

Cheriot/Types.v
@@ -1,137 +1,130 @@
 Require Import Kami.AllNotations ProcKami.Cheriot.Lib.
 Require Import RecordUpdate.RecordUpdate.
-  
-Section CapAccessors.
-  Variable CapSz: nat.
-  Variable AddrSz: nat.
+Require Export ProcKami.Cheriot.CheriotTypes.
 
-  Definition CapPerms :=
-    STRUCT_TYPE {
-        "U0" :: Bool;
-        "SE" :: Bool; (* Permit Seal *)
-        "US" :: Bool; (* Permit Unseal *)
-        "EX" :: Bool; (* Permit Execute *)
-        "SR" :: Bool; (* Permit system register access *)
-        "MC" :: Bool; (* Permit Load or Store of Caps *)
-        "LD" :: Bool; (* Permit Load *)
-        "SL" :: Bool; (* Permit Store of Local *)
-        "LM" :: Bool; (* Permit Mutability of loaded cap, i.e. allow store using the cap *)
-        "SD" :: Bool; (* Permit Store *)
-        "LG" :: Bool; (* Permit Store into Global of loaded cap *)
-        "GL" :: Bool }. (* Global *)
+Section Roots.
+  Section Ty.
+    Variable ty: Kind -> Type.
+    Local Open Scope kami_expr.
+    Definition RootT := Z.pow 2 (Z.of_nat (CapBTSz - 1)).
+    Definition ExecRootPermExpr : CapPerms @# ty := (Const ty (getDefaultConst CapPerms))
+                                                      @%[ "GL" <- $$true ]
+                                                      @%[ "EX" <- $$true ]
+                                                      @%[ "LD" <- $$true ]
+                                                      @%[ "MC" <- $$true ]
+                                                      @%[ "LG" <- $$true ]
+                                                      @%[ "LM" <- $$true ]
+                                                      @%[ "SR" <- $$true ].
 
-  Record CapAccessors := {
-      CapRSz: nat;
-      getCapR: forall ty, Bit CapSz @# ty -> Bit CapRSz @# ty;
-      setCapR: forall ty, Bit CapRSz @# ty -> Bit CapSz @# ty -> Bit CapSz @# ty;
-      CapPSz: nat;
-      getCapP: forall ty, Bit CapSz @# ty -> Bit CapPSz @# ty;
-      setCapP: forall ty, Bit CapPSz @# ty -> Bit CapSz @# ty -> Bit CapSz @# ty;
-      CapOTypeSz: nat;
-      getCapOType: forall ty, Bit CapSz @# ty -> Bit CapOTypeSz @# ty;
-      setCapOType: forall ty, Bit CapOTypeSz @# ty -> Bit CapSz @# ty -> Bit CapSz @# ty;
-      CapESz: nat;
-      getCapE: forall ty, Bit CapSz @# ty -> Bit CapESz @# ty;
-      setCapE: forall ty, Bit CapESz @# ty -> Bit CapSz @# ty -> Bit CapSz @# ty;
-      CapBSz: nat;
-      getCapB: forall ty, Bit CapSz @# ty -> Bit CapBSz @# ty;
-      setCapB: forall ty, Bit CapBSz @# ty -> Bit CapSz @# ty -> Bit CapSz @# ty;
-      CapTSz: nat;
-      getCapT: forall ty, Bit CapSz @# ty -> Bit CapTSz @# ty;
-      setCapT: forall ty, Bit CapTSz @# ty -> Bit CapSz @# ty -> Bit CapSz @# ty;
-      getCapEFromExp: forall ty, Bit (Nat.log2_up AddrSz) @# ty -> Bit CapESz @# ty;
-      getCapExpFromE: forall ty, Bit CapESz @# ty -> Bit (Nat.log2_up AddrSz) @# ty;
-      isSealed: forall ty, Bit CapSz @# ty -> Bool @# ty;
-      isSentry: forall ty, Bit CapSz @# ty -> Bool @# ty;
-      isIeSentry: forall ty, Bit CapSz @# ty -> Bool @# ty;
-      isIdSentry: forall ty, Bit CapSz @# ty -> Bool @# ty;
-      getOTypeFromIe: forall ty, Bool @# ty (* Interrupt Enabled ? *) -> Bit CapOTypeSz @# ty;
-      seal: forall ty, Bit CapOTypeSz @# ty -> Bit CapSz @# ty -> Bit CapSz @# ty;
-      unseal: forall ty, Bit CapSz @# ty -> Bit CapSz @# ty;
-      isSealAddr: forall ty, Bit AddrSz @# ty -> Bool @# ty (* Exec seal or not *) -> Bool @# ty;
-      getCapPerms: forall ty, Bit CapSz @# ty -> CapPerms ## ty;
-      setCapPerms: forall ty, CapPerms @# ty -> Bit CapSz @# ty -> Bit CapSz ## ty;
-      BaseTop := STRUCT_TYPE {
-                     "base" :: Bit AddrSz;
-                     "top"  :: Bit (AddrSz + 1);
-                     "aTopBase" :: Bit (AddrSz - CapBSz) };
-      getCapBaseTop: forall ty, Bit CapSz @# ty -> Bit AddrSz @# ty -> BaseTop ## ty;
-      CapBounds := STRUCT_TYPE {
-                       "B" :: Bit CapBSz;
-                       "T" :: Bit CapTSz;
-                       "exp" :: Bit (Nat.log2_up AddrSz);
-                       "exact?" :: Bool };
-      getCapBounds: forall ty, Bit AddrSz @# ty (* Base *) -> Bit AddrSz @# ty (* Length *) -> CapBounds ## ty;
-      setCapBounds ty (cap: Bit CapSz @# ty) B T exp :=
-        setCapE (getCapEFromExp exp) (setCapT T (setCapB B cap));
-      ExpandedCap := STRUCT_TYPE {
-                         "R"     :: Bit CapRSz ;
-                         "p"     :: CapPerms;
-                         "oType" :: Bit CapOTypeSz;
-                         "base"  :: Bit AddrSz ;
-                         "top"   :: Bit (AddrSz + 1) };
-      getCapFromExpanded ty (ec: ExpandedCap @# ty) :=
-        ( LETC lenFull <- (ec @% "top") - ZeroExtend 1 (ec @% "base");
-          LETC lenFullMsb <- unpack Bool (UniBit (TruncMsb AddrSz 1) #lenFull);
-          LETC lenLsb <- UniBit (TruncLsb AddrSz 1) #lenFull;
-          LETC len <- ITE #lenFullMsb $$(wones AddrSz) #lenLsb;
-          LETE capBounds <- @getCapBounds ty (ec @% "base") #len;
-          LETC initCap <- setCapOType (ec @% "oType") (setCapR (ec @% "R") ($$(getDefaultConst (Bit CapSz))));
-          LETE permCap <- setCapPerms (ec @% "p") #initCap;
-          RetE (setCapBounds #permCap (#capBounds @% "B") (#capBounds @% "T") (#capBounds @% "exp")))%kami_expr;
-      getExpandedFromCap ty (c: Bit CapSz @# ty) (addr: Bit AddrSz @# ty) :=
-        ( LETE perms <- getCapPerms c;
-          LETE baseTop <- getCapBaseTop c addr;
-          RetE (STRUCT { "R"     ::= getCapR c;
-                         "p"     ::= #perms;
-                         "oType" ::= getCapOType c;
-                         "base"  ::= #baseTop @% "base";
-                         "top"   ::= #baseTop @% "top" } : ExpandedCap @# ty) )%kami_expr
-    }.
-End CapAccessors.
+    Definition DataRootPermExpr : CapPerms @# ty := (Const ty (getDefaultConst CapPerms))
+                                                      @%[ "GL" <- $$true ]
+                                                      @%[ "LD" <- $$true ]
+                                                      @%[ "SD" <- $$true ]
+                                                      @%[ "MC" <- $$true ]
+                                                      @%[ "SL" <- $$true ]
+                                                      @%[ "LG" <- $$true ]
+                                                      @%[ "LM" <- $$true ].
 
-Inductive Extension := Base | M.
+    Definition SealRootPermExpr : CapPerms @# ty := (Const ty (getDefaultConst CapPerms))
+                                                      @%[ "GL" <- $$true ]
+                                                      @%[ "SE" <- $$true ]
+                                                      @%[ "US" <- $$true ]
+                                                      @%[ "U0" <- $$true ].
+
+    Definition ExecRootCapExpr: Cap @# ty := STRUCT { "R" ::= $0;
+                                                      "p" ::= encodePerms ExecRootPermExpr;
+                                                      "oType" ::= $0;
+                                                      "E" ::= $$(wones CapESz);
+                                                      "T" ::= $$(ZToWord CapBTSz RootT);
+                                                      "B" ::= $0 }.
+ 
+    Definition DataRootCapExpr: Cap @# ty := ExecRootCapExpr @%[ "p" <- encodePerms DataRootPermExpr ].
+    Definition SealRootCapExpr: Cap @# ty := ExecRootCapExpr @%[ "p" <- encodePerms SealRootPermExpr ].
+  End Ty.
+
+  Definition ExecRootPerm : type (Bit CapPermSz) := evalExpr (encodePerms (ExecRootPermExpr _)).
+  Definition DataRootPerm : type (Bit CapPermSz) := evalExpr (encodePerms (DataRootPermExpr _)).
+  Definition SealRootPerm : type (Bit CapPermSz) := evalExpr (encodePerms (SealRootPermExpr _)).
+  Definition ExecRootCap : type Cap := evalExpr (ExecRootCapExpr _).
+  Definition DataRootCap : type Cap := evalExpr (DataRootCapExpr _).
+  Definition SealRootCap : type Cap := evalExpr (SealRootCapExpr _).
+End Roots.
+
+Definition mkFullCap ty (cap: Cap @# ty) (val: Data @# ty) : FullCap @# ty :=
+  (STRUCT { "cap" ::= cap ; "val" ::= val })%kami_expr.
+
+Section ValidInits.
+  Local Open Scope kami_expr.
+  Definition PccValid (pcCap: type Cap) :=
+    evalLetExpr ( LETC perms <- getCapPerms ###pcCap;
+                  RetE (###perms @% "EX" && !(isCapSealed ###pcCap))) = true.
+
+  Definition MtccValid (mtccCap: type Cap) (mtccVal: type Addr) mtccSize :=
+    evalLetExpr ( LETC perms <- getCapPerms ###mtccCap;
+                  LETC sealed <- isCapSealed ###mtccCap;
+                  LETC aligned <- isZero (UniBit (TruncLsb 2 _) ###mtccVal);
+                  LETE baseTop <- getCapBaseTop (STRUCT {"cap" ::= ###mtccCap; "val" ::= ###mtccVal});
+                  LETC baseBound <- ###mtccVal >= (###baseTop @% "base");
+                  LETC topBound <- (ZeroExtend 1 ###mtccVal + $mtccSize <= (###baseTop @% "top"));
+                  RetE ((###perms @% "EX") && (###perms @% "SR") && !###sealed && ###aligned
+                        && (###baseBound && ###topBound))) = true.
+
+  Definition MtdcValid (mtdcCap: type Cap) (mtdcVal: type Addr) numProcesses :=
+    evalLetExpr ( LETE baseTop <- getCapBaseTop (STRUCT {"cap" ::= ###mtdcCap; "val" ::= ###mtdcVal});
+                  LETC baseBound <- ###mtdcVal >= (###baseTop @% "base");
+                  LETC topBound <- (ZeroExtend 1 ###mtdcVal +
+                                      Const type (ZToWord _ (16 + (Z.of_nat (numProcesses*NumBanks*NumRegs))))
+                                    <= (###baseTop @% "top"));
+                  RetE (###baseBound && ###topBound)) = true.
+End ValidInits.
 
 Theorem Extension_eq_dec: forall (e1 e2: Extension), {e1 = e2} + {e1 <> e2}.
 Proof.
   decide equality.
 Qed.
 
-Section VarType.
-  Local Notation "## x" := (Var type (SyntaxKind _) x) (no associativity, at level 0).
+Definition Inst := Bit InstSz.
+Definition CompInst := Bit CompInstSz.
+Definition RegId := Bit RegIdSz.
+Definition ScrId := Bit ScrIdSz.
 
-  Local Open Scope kami_expr.
-  Definition PcCapValid Xlen CapSz (capAccessors: CapAccessors CapSz Xlen) (pcCap: word CapSz) :=
-    evalLetExpr (LETE perms <- getCapPerms capAccessors (Const type pcCap);
-                 RetE (##perms @% "EX")) = true /\
-      evalExpr ((isSealed capAccessors (Const _ pcCap))) = false.
+Definition isInstNotCompressed ty sz (bitString : Bit sz @# ty) := isNotZero (ZeroExtendTruncLsb 2 bitString).
 
-  Definition PcValValid Xlen (pcAddr: word Xlen) (compressed: bool) :=
-    compressed = false -> truncLsb pcAddr = ZToWord 2 0.
-  Definition PccValid Xlen CapSz (capAccessors: CapAccessors CapSz Xlen) (pcCap: word CapSz) (pcAddr: word Xlen)
-    (compressed: bool) :=
-    PcCapValid capAccessors pcCap /\ PcValValid pcAddr compressed.
+Definition isInstCompressed ty sz (bitString : Bit sz @# ty) := isZero (ZeroExtendTruncLsb 2 bitString).
 
-  Definition MtccValid Xlen CapSz (capAccessors: CapAccessors CapSz Xlen)
-    (mtccCap: word CapSz) (mtccVal: word Xlen) :=
-    evalLetExpr ( LETE perms <- getCapPerms capAccessors (Const type mtccCap);
-                  LETC sealed <- isSealed capAccessors (Const type mtccCap);
-                  LETC aligned <- isZero (ZeroExtendTruncLsb 2 (Const type mtccVal));
-                  LETE baseTop <- getCapBaseTop capAccessors (Const type mtccCap) (Const type mtccVal);
-                  LETC baseBound <- Const type mtccVal >= (##baseTop @% "base");
-                  LETC topBound <- (ZeroExtend 1 (Const type mtccVal) + Const type (natToWord _ 4) <=
-                                      (##baseTop @% "top"));
-                  RetE ((##perms @% "EX") && (##perms @% "SR") && !##sealed && ##aligned
-                        && (##baseBound && ##topBound))) = true.
+Definition IeInit := false.
+Definition MeieInit := false.
+Definition MtieInit := false.
+Definition MsieInit := false.
 
-  Definition MtdcValid Xlen CapSz (capAccessors: CapAccessors CapSz Xlen)
-    (mtdcCap: word CapSz) (mtdcVal: word Xlen) :=
-    evalLetExpr ( LETE baseTop <- getCapBaseTop capAccessors (Const type mtdcCap) (Const type mtdcVal);
-                  LETC baseBound <- Const type mtdcVal >= (##baseTop @% "base");
-                  LETC topBound <- (ZeroExtend 1 (Const type mtdcVal) + Const type (natToWord _ 8) <=
-                                      (##baseTop @% "top"));
-                  RetE (##baseBound && ##topBound)) = true.  
-End VarType.
+Definition isMemAscii := false.
+Definition isMemRfArg := true.
+Definition isRegsAscii := false.
+Definition isRegsRfArg := true.
+Definition pcCapReg := "pcCap".
+Definition pcValReg := "pcVal".
+Definition prevPcCapReg := "prevPcCap".
+Definition prevPcValReg := "prevPcVal".
+Definition justFenceIReg := "justFenceI".
+Definition startFenceIReg := "startFenceI".
+Definition reqJustFenceIReg := "reqJustFenceI".
+Definition tagRead := "tagRead".
+Definition tagWrite := "tagWrite".
+Definition tagArray := "tagArray".
+Definition regsRead1 := "regsRead1".
+Definition regsRead2 := "regsRead2".
+Definition regsWrite := "regsWrite".
+Definition regsArray := "regsArray".
+Definition regsRfString := "regsArrayFileArg".
+Definition memArray := "memArray".
+Definition mtccReg := "MTCC".
+Definition mtdcReg := "MTDC".
+Definition mScratchCReg := "MScratchC".
+Definition mepccReg := "MEPCC".
+Definition mStatusReg := "MStatus".
+Definition mieReg := "MIE".
+Definition mCauseReg := "MCause".
+Definition mtValReg := "MTVal".
 
 Record MemBankInit :=
   { instRqName: string;
@@ -140,456 +133,321 @@ Record MemBankInit :=
     memArrayName: string;
     memRfString: string }.
 
-Class ProcParams :=
-  { Xlen: nat;
-    xlenIs32_or_64: Xlen = 32 \/ Xlen = 64;
-    CapSz := Xlen;
-    capAccessors: CapAccessors CapSz Xlen;
-    PcCap: word CapSz;
-    PcAddr: word Xlen;
-    compressed: bool;
-    pccValid: PccValid capAccessors PcCap PcAddr compressed;
-    ExecRootCap: word CapSz;
-    DataRootCap: word CapSz;
-    SealRootCap: word CapSz;
-    MtccVal: word Xlen;
-    MtdcVal: word Xlen;
-    IeInit: bool;
-    MeieInit: bool;
-    MtieInit: bool;
-    MsieInit: bool;
-    supportedExts: list Extension;
-    extsHasBase: In Base supportedExts;
-    RegIdSz: nat;
-    regIdSzIs4_or5: RegIdSz = 4 \/ RegIdSz = 5;
+Definition prefixHex x n := (x ++ "_" ++ natToHexStr n)%string.
+
+Definition createMemRFParam (n: nat) : MemBankInit :=
+  {|instRqName := prefixHex "instRq" n;
+    loadRqName := prefixHex "loadRq" n;
+    storeRqName := prefixHex "storeRq" n;
+    memArrayName := prefixHex memArray n;
+    memRfString := prefixHex "memArrayFileArg" n |}.
+
+Definition memBankInits := map createMemRFParam (zeroToN 8).
+
+Theorem lengthMemBankInits: length memBankInits = NumBanks.
+Proof.
+  reflexivity.
+Qed.
+
+Class MemParams := {
     LgNumMemBytes: nat;
     (* NumMemBytes denotes the number of bytes in each bank. So total physical memory = NumMemBytes * NumBanks *)
     NumMemBytes := Nat.pow 2 LgNumMemBytes;
-    memBankInits: list MemBankInit;
-    NumBanks := (Xlen + CapSz) / 8;
-    lengthMemBankInits: length memBankInits = NumBanks;
-    isMemAscii: bool;
-    isMemRfArg: bool;
-    memInit: Fin.t (NumMemBytes * NumBanks) -> word 8;
-    procName: string;
-    pcCapReg: string;
-    pcValReg: string;
-    prevPcCapReg: string;
-    prevPcValReg: string;
-    justFenceIReg: string;
-    startFenceIReg: string;
-    reqJustFenceIReg: string;
-    tagRead: string;
-    tagWrite: string;
-    tagArray: string;
-    memArray: string;
-    regsRead1: string;
-    regsRead2: string;
-    regsWrite: string;
-    regsArray: string;
-    Data := Bit Xlen;
-    Cap := Bit CapSz;
-    FullCapWithTag := STRUCT_TYPE { "tag" :: Bool;
-                                    "cap" :: Cap;
-                                    "val" :: Data };
-    isRegsAscii: bool;
-    isRegsRfArg: bool;
-    regsRfString: string;
-    regsInit: Fin.t (Nat.pow 2 RegIdSz) -> ConstT FullCapWithTag;
-    hasTrap: bool }.
+    memInit: Fin.t (Nat.pow 2 LgNumMemBytes * 8) -> word 8 }.
 
-Section ParamDefinitions.
-  Context {procParams: ProcParams}.
+Class CoreConfigParams := {
+    procName : string;
+    numProcesses: nat;
+    hasTrap: bool;
+    memParams: MemParams;
+    regsInit: Fin.t 32 -> type FullCapWithTag;
+    pcCapInit: type Cap;
+    pcValInit: word 30;
+    pccValidThm: PccValid pcCapInit;
+    mtccValInit: word 30;
+    mtccSize: nat;
+    mtccValidThm: MtccValid ExecRootCap (wcombine mtccValInit (wzero 2)) mtccSize;
+    mtdcValInit: word 30;
+    mtdcValidThm: MtdcValid DataRootCap (wcombine mtdcValInit (wzero 2)) numProcesses }.
 
-  Definition Addr := Bit Xlen.
+Record InstProperties :=
+  { hasCs1      : bool ;
+    hasCs2      : bool ;
+    hasCd       : bool ;
+    hasScr      : bool ;
+    hasCsr      : bool ;
+    implicitReg : nat ;
+    implicitScr : nat ;
+    implicitCsr : word (snd immField);
+    signExt     : bool;
+    isLoad      : bool ;
+    isStore     : bool }.
 
-  Definition FullCap :=
-    STRUCT_TYPE { "cap" :: Cap;
-                  "val" :: Data }.
+Global Instance InstPropertiesEtaX : Settable _ :=
+  settable!
+    Build_InstProperties
+  < hasCs1 ; hasCs2 ; hasCd; hasScr ; hasCsr ; implicitReg ; implicitScr ; implicitCsr ;
+signExt ; isLoad ; isStore  >.
 
-  Section Ty.
+Definition DefProperties :=
+  {|hasCs1      := false ;
+    hasCs2      := false ;
+    hasCd       := true ;
+    hasScr      := false ;
+    hasCsr      := false ;
+    implicitReg := 0 ;
+    implicitScr := 0 ;
+    implicitCsr := wzero _ ;
+    signExt     := true ;
+    isLoad      := false ;
+    isStore     := false |}.
+
+Definition FieldRange := {x: (nat * nat) & word (snd x)}.
+Definition UniqId := (list FieldRange)%type.
+
+Section Match.
+  Variable ty: Kind -> Type.
+  Local Open Scope kami_expr.
+
+  Variable inst: Inst @# ty.
+
+  Definition matchField (f: FieldRange) :=
+    let '(existT (start, size) field) := f in
+    UniBit (TruncMsb start size) (ZeroExtendTruncLsb (start + size) inst) ==
+      Const ty field.
+
+  Definition matchUniqId (uid: UniqId) :=
+    CABool And (map matchField uid).
+End Match.
+
+Definition fieldVal range value : FieldRange :=
+  existT (fun x => word (snd x)) range value.
+
+Record ImmEncoder := {
+    instPos : nat;
+    immPos  : list (nat * nat) }.
+
+Definition immFieldWidth (enc: ImmEncoder) :=
+  (instPos enc, fold_right (fun '(_, val) accum => val + accum) 0 (immPos enc)).
+
+Definition isGoodInstEncode (uniqId: UniqId) (immEncoder: list ImmEncoder)
+  (instProperties: InstProperties) :=
+  getDisjointContiguous
+    ((if hasCs1 instProperties then [rs1FixedField] else []) ++
+       (if hasCs2 instProperties then [rs2FixedField] else []) ++
+       (if hasCd instProperties then [rdFixedField] else []) ++
+       (if hasScr instProperties then [rs2FixedField] else []) ++
+       (if hasCsr instProperties then [immField] else []) ++
+       map (@projT1 _ _) uniqId ++
+       map immFieldWidth immEncoder) = Some (snd instSizeField, InstSz).
+
+Definition LdOp := 0.
+Definition StOp := 1.
+Definition MemOpSz := 1.
+
+Definition MemSizeSz := (Nat.log2_up NumBanks) + 1.
+Definition MemSize := Bit MemSizeSz.
+
+Definition MemOpInfo :=
+  STRUCT_TYPE {
+      "op"    :: Bit MemOpSz;
+      "size"  :: MemSize;
+      "MC"    :: Bool;
+      "LM"    :: Bool;
+      "LG"    :: Bool;
+      "sign?" :: Bool;
+      "cap?"  :: Bool }.
+
+Goal size MemOpInfo <= CapSz.
+Proof.
+  unfold MemOpInfo, MemOpSz, CapSz.
+  simpl.
+  lia.
+Qed.
+
+Definition FullOutput :=
+  STRUCT_TYPE {
+      "wb?" :: Bool;
+      "cdTag" :: Bool;
+      "cdCap" :: Cap;
+      "cdVal" :: Data;
+      "taken?" :: Bool;
+      "pcMemAddr" :: Addr;
+      "changePcCap?" :: Bool;
+      "pcCap" :: Cap;
+      "changeIe?" :: Bool;
+      "newIe" :: Bool;
+      "exception?" :: Bool;
+      "exceptionCause" :: Data;
+      "exceptionValue" :: Addr;
+      "baseException?" :: Bool;
+      "pcCapException?" :: Bool;
+      "mem?" :: Bool;
+      "memCap?" :: Bool;
+      "memSize" :: MemSize;
+      "store?" :: Bool;
+      "ldSigned?" :: Bool;
+      "ldPerms" :: CapPerms;
+      "fenceI?" :: Bool;
+      "wbScr?" :: Bool;
+      "scrTag" :: Bool;
+      "scrCap" :: Cap;
+      "scrVal" :: Data;
+      "scrException?" :: Bool;
+      "wbCsr?" :: Bool;
+      "csrVal" :: Data }.
+
+Section ReadArray.
+  Variable ty: Kind -> Type.
+  Variable addr: Addr @# ty.
+  Variable n: nat.
+  Variable arr: Array n (Bit 8) @# ty.
+  Local Open Scope kami_expr.
+  Definition readArrayConstSize (size: nat) :=
+    BuildArray (fun (i: Fin.t size) => arr@[addr + $(FinFun.Fin2Restrict.f2n i)]).
+End ReadArray.
+
+Section InstEntry.
+  Variable ik: Kind.
+  Record InstEntry :=
+    { instName       : string;
+      uniqId         : UniqId;
+      immEncoder     : list ImmEncoder;
+      spec           : forall ty, FullCap @# ty -> Inst @# ty ->
+                                  FullCapWithTag @# ty -> FullCapWithTag @# ty ->
+                                  FullCapWithTag @# ty -> Data @# ty -> ik ## ty;
+      instProperties : InstProperties;
+      goodInstEncode : isGoodInstEncode uniqId immEncoder instProperties;
+      immStart       : nat;
+      immEnd         : nat;
+      goodImmEncode  : getDisjointContiguous (concat (map immPos immEncoder)) = Some (immStart, immEnd)
+    }.
+
+  Record InstEntryFull := {
+      xlens : list nat;
+      extension: Extension;
+      instEntries: list InstEntry }.
+
+  Section Encoder.
+    Variable i: InstEntry.
+    Variable cs1 cs2 cd: word (snd rs1FixedField).
+    Variable csr: word (snd immField).
+    Variable immV: word Xlen.
+    Fixpoint encodeImmField (imms: list (nat * nat)) :=
+      match imms return word (fold_right (fun '(_, val) sum => sum + val) 0 imms) with
+      | nil => WO
+      | (start, width) :: xs => wcombine (encodeImmField xs) (extractWord immV start width)
+      end.
+
+    Definition encodeFullInstList :=
+      uniqId i ++
+        map (fun ie => existT _ (instPos ie, _) (encodeImmField (immPos ie))) (immEncoder i) ++
+        (if hasCs1 (instProperties i) then [existT _ rs1FixedField cs1] else []) ++
+        (if hasCs2 (instProperties i) then [existT _ rs2FixedField cs2] else []) ++
+        (if hasCd (instProperties i) then [existT _ rdFixedField cd] else []) ++
+        (if hasScr (instProperties i) then [existT _ rs2FixedField cs2] else []) ++
+        (if hasCsr (instProperties i) then [existT _ immField csr] else []).
+
+    Definition encodeInst := @truncLsb InstSz _ ((wordCombiner (2'b"11") (SigWordSort.sort encodeFullInstList))).
+  End Encoder.
+
+  Section Decoder.
+    Variable inst: word InstSz.
+    Fixpoint immDecoderHelp (instStart: nat) (ls: list (nat * nat)) : list FieldRange :=
+      match ls with
+      | nil => nil
+      | (immStart, width) :: xs => existT _ (immStart, width) (extractWord inst instStart width) ::
+                                     immDecoderHelp (instStart + width) xs
+      end.
+
+    Definition immDecoder (immEnc: ImmEncoder) :=
+      immDecoderHelp (instPos immEnc) (immPos immEnc).
+
+    Variable i: InstEntry.
+
+    Definition decodePartialImmList :=
+      SigWordSort.sort (concat (map immDecoder (immEncoder i))).
+
+    Definition decodeImm: word Xlen :=
+      match decodePartialImmList with
+      | nil => wzero Xlen
+      | existT (start, _) _ :: _ =>
+          let res := wordCombiner (wzero start) decodePartialImmList in
+          wconcat
+            (if (andb (signExt (instProperties i)) (weqb (get_msb res) WO~1))
+             then wones _
+             else wzero (Xlen - (fold_right (fun new sum => sum + snd (projT1 new)) start decodePartialImmList)))
+            res
+      end.
+  End Decoder.
+
+  Section DecoderExpr.
     Variable ty: Kind -> Type.
-    Local Open Scope kami_expr.
-    Definition mkFullCap (cap : Cap @# ty) (val : Data @# ty) :=
-      STRUCT { "cap" ::= cap;
-               "val" ::= val }.
+    Variable inst: Inst @# ty.
+    Fixpoint immDecIntervalHelp (instStart: nat) (ls: list (nat * nat)) : list (nat * (nat * nat)) :=
+      match ls with
+      | nil => nil
+      | (immStart, width) :: xs => (immStart, (instStart, width)) :: immDecIntervalHelp (instStart + width) xs
+      end.
 
-    Definition mkFullCapWithTag (tag : Bool @# ty) (cap : Cap @# ty)
-      (val : Data @# ty) :=
-      STRUCT { "tag" ::= tag;
-               "cap" ::= cap;
-               "val" ::= val }.
-  End Ty.
+    Definition immDecInterval (immEnc: ImmEncoder) :=
+      immDecIntervalHelp (instPos immEnc) (immPos immEnc).
 
-  Section InstEncoding.
-    Definition RegId := Bit RegIdSz.
-    Definition RegFixedIdSz := 5.
-    Definition NumRegs := 2^RegIdSz.
-    Definition InstSz := 32.
-    Definition Inst := (Bit InstSz).
-    Definition CompInstSz := 16.
-    Definition CompInst := (Bit CompInstSz).
-    Definition ScrIdSz := 5.
-    Definition ScrId := Bit ScrIdSz.
+    Variable i: InstEntry.
 
-    Definition isInstNotCompressed ty sz (bitString : Bit sz @# ty)
-      := unpack Bool (UniBit (UAnd _) (ZeroExtendTruncLsb 2 bitString)).
+    Definition decIntervals :=
+      SigTripleSort.sort (concat (map immDecInterval (immEncoder i))).
 
-    Definition isInstCompressed ty sz (bitString : Bit sz @# ty) :=
-      (!(isInstNotCompressed (bitString)))%kami_expr.
+    Definition decExprs := map (fun x =>
+                                  existT (fun y => Bit (snd y) @# ty)
+                                    (fst x, snd (snd x))
+                                    (extractFieldExprDynamicWidth inst (fst (snd x)) (snd (snd x))))
+                             decIntervals.
 
-    Definition instSizeField := (0, 2).
-    Definition opcodeField := (2, 5).
-    Definition funct3Field := (12, 3).
-    Definition funct7Field := (25, 7).
-    Definition funct6Field := (26, 6).
-    Definition immField := (20, 12).
-    Definition rs1Field := (15, RegIdSz).
-    Definition rs2Field := (20, RegIdSz).
-    Definition rdField := (7, RegIdSz).
-    Definition rs1FixedField := (15, RegFixedIdSz).
-    Definition rs2FixedField := (20, RegFixedIdSz).
-    Definition rdFixedField := (7, RegFixedIdSz).
-    Definition auiLuiField := (12, 20).
+    Definition decodeImmExpr :=
+      match decExprs with
+      | nil => Const ty (wzero Xlen)
+      | (existT (start, _) _) :: _ =>
+          let res := bitsCombiner (Const ty (wzero start)) decExprs in
+          if signExt (instProperties i)
+          then SignExtendTruncLsb Xlen res
+          else ZeroExtendTruncLsb Xlen res
+      end.
+  End DecoderExpr.
+End InstEntry.
 
-    Definition imm12   := [(0, 12)].
-    Definition imm5    := [(0, 5)].
-    Definition imm20_U := [(12, 20)].
-    Definition imm20_J := [(12, 8); (11, 1); (1, 10); (20, 1)].
-    Definition imm6    := [(0, 6)].
-    Definition imm7    := [(5, 7)].
-    Definition imm5_B  := [(11, 1); (1, 4)].
-    Definition imm7_B  := [(5, 6); (12, 1)].
+Record FuncEntryFull :=
+  { funcNameFull        : string;
+    localFuncInputFull  : Kind;
+    localFuncFull       : forall ty, localFuncInputFull @# ty -> FullOutput ## ty;
+    instsFull           : list (InstEntryFull localFuncInputFull) }.
 
-    Section Fields.
-      Variable ty: Kind -> Type.
-      Variable inst: Inst @# ty.
+Record FuncEntry :=
+  { funcName        : string;
+    localFuncInput  : Kind;
+    localFunc       : forall ty, localFuncInput @# ty -> FullOutput ## ty;
+    insts           : list (InstEntry localFuncInput) }.
 
-      Local Open Scope kami_expr.
+Definition filterInsts k (ls: list (InstEntryFull k)) :=
+  fold_right (fun new rest =>
+                (if (getBool (in_dec Nat.eq_dec Xlen (xlens new)) &&
+                       getBool (in_dec Extension_eq_dec (extension new) supportedExts))%bool
+                 then instEntries new
+                 else []) ++ rest) [] ls.
 
-      Notation extractFieldFromInst span := (extractFieldExpr InstSz inst (fst span) (snd span)).
+Definition mkFuncEntry (fe : FuncEntryFull) :=
+  {|funcName := funcNameFull fe;
+    localFuncInput := localFuncInputFull fe;
+    localFunc := localFuncFull fe;
+    insts := filterInsts (instsFull fe)
+  |}.
 
-      Notation extractFieldFromInstDynamic span := (extractFieldExprDynamicWidth inst (fst span) (snd span)).
-      
-      Definition instSize := extractFieldFromInst instSizeField.
-      Definition opcode := extractFieldFromInst opcodeField.
-      Definition funct3 := extractFieldFromInst funct3Field.
-      Definition funct7 := extractFieldFromInst funct7Field.
-      Definition funct6 := extractFieldFromInst funct6Field.
-      Definition imm := extractFieldFromInst immField.
-      Definition branchOffset := ({< extractFieldFromInst (31, 1),
-                                     extractFieldFromInst ( 7, 1),
-                                     extractFieldFromInst (25, 6),
-                                     extractFieldFromInst ( 8, 4), $$(WO~0) >}).
-      Definition jalOffset := ({< extractFieldFromInst (31,  1),
-                                  extractFieldFromInst (12,  8),
-                                  extractFieldFromInst (20,  1),
-                                  extractFieldFromInst (21, 10), $$(WO~0) >}).
-      Definition auiLuiOffset := extractFieldFromInst auiLuiField.
-      Definition rs1 := extractFieldFromInstDynamic rs1Field.
-      Definition rs2 := extractFieldFromInstDynamic rs2Field.
-      Definition rd := extractFieldFromInstDynamic rdField.
-      Definition rs1Fixed := extractFieldFromInst rs1FixedField.
-      Definition rs2Fixed := extractFieldFromInst rs2FixedField.
-      Definition rdFixed := extractFieldFromInst rdFixedField.
-    End Fields.
+Record ScrReg :=
+  { scrRegInfo    : RegInfo RegFixedIdSz;
+    isLegal       : forall ty, Data @# ty -> Bool @# ty;
+    legalize      : forall ty, Data @# ty -> Data @# ty }.
 
-    Record InstProperties :=
-      { hasCs1      : bool ;
-        hasCs2      : bool ;
-        hasCd       : bool ;
-        hasScr      : bool ;
-        hasCsr      : bool ;
-        implicitReg : nat ;
-        implicitScr : nat ;
-        implicitCsr : word (snd immField);
-        signExt     : bool;
-        isLoad      : bool ;
-        isStore     : bool }.
-
-    Global Instance InstPropertiesEtaX : Settable _ :=
-      settable!
-        Build_InstProperties
-      < hasCs1 ; hasCs2 ; hasCd; hasScr ; hasCsr ; implicitReg ; implicitScr ; implicitCsr ;
-        signExt ; isLoad ; isStore  >.
-    
-    Definition DefProperties :=
-      {|hasCs1      := false ;
-        hasCs2      := false ;
-        hasCd       := true ;
-        hasScr      := false ;
-        hasCsr      := false ;
-        implicitReg := 0 ;
-        implicitScr := 0 ;
-        implicitCsr := wzero _ ;
-        signExt     := true ;
-        isLoad      := false ;
-        isStore     := false |}.
-
-    Definition FieldRange := {x: (nat * nat) & word (snd x)}.
-    Definition UniqId := (list FieldRange)%type.
-
-    Definition fieldVal range value : FieldRange :=
-      existT (fun x => word (snd x)) range value.
-
-    Record ImmEncoder := {
-        instPos : nat;
-        immPos  : list (nat * nat) }.
-
-    Definition immFieldWidth (enc: ImmEncoder) :=
-      (instPos enc, fold_right (fun '(_, val) accum => val + accum) 0 (immPos enc)).
-
-    Definition isGoodInstEncode (uniqId: UniqId) (immEncoder: list ImmEncoder)
-      (instProperties: InstProperties) :=
-      getDisjointContiguous
-        ((if hasCs1 instProperties then [rs1FixedField] else []) ++
-           (if hasCs2 instProperties then [rs2FixedField] else []) ++
-           (if hasCd instProperties then [rdFixedField] else []) ++
-           (if hasScr instProperties then [rs2FixedField] else []) ++
-           (if hasCsr instProperties then [immField] else []) ++
-           map (@projT1 _ _) uniqId ++
-           map immFieldWidth immEncoder) = Some (snd instSizeField, InstSz).
-  End InstEncoding.
-
-  Definition CapException        := N.to_nat (hex "1c").
-  Definition CapBoundsViolation  := 1.  (* Reg/PC *)
-  Definition CapTagViolation     := 2.  (* Reg *)
-  Definition CapSealViolation    := 3.  (* Reg *)
-  Definition CapExecViolation    := 17. (* Reg *)
-  Definition CapLdViolation      := 18. (* Reg *)
-  Definition CapStViolation      := 19. (* Reg *)
-  Definition CapStCapViolation   := 21. (* Reg *)
-  Definition CapStLocalViolation := 22. (* Reg *)
-  Definition CapSysRegViolation  := 24. (* PC *)
-  Definition CapLdMisaligned     := 4.  (* Addr *)
-  Definition CapStMisaligned     := 6.  (* Addr *)
-
-  Definition InstMisaligned      := 0.  (* Addr *)
-  Definition InstAccessFault     := 1.  (* Addr *)
-  Definition InstPageFault       := 12. (* Addr *)
-  Definition LoadAccessFault     := 5.  (* Addr *)
-  Definition LoadPageFault       := 13. (* Addr *)
-  Definition StoreAccessFault    := 7.  (* Addr *)
-  Definition StorePageFault      := 15. (* Addr *)
-  Definition TagAccessFault      := 24. (* Addr *)
-  Definition TagPageFault        := 25. (* Addr *)
-  Definition InstIllegal         := 2.  (* Inst *)
-  Definition ECall               := 8.
-
-  Definition LdOp := 0.
-  Definition StOp := 1.
-  Definition MemOpSz := 1.
-
-  Definition MemSizeSz := (Nat.log2_up ((Xlen + CapSz)/8)) + 1.
-  Definition MemSize := Bit MemSizeSz.
-
-  Definition MemOpInfo :=
-    STRUCT_TYPE {
-        "op"    :: Bit MemOpSz;
-        "size"  :: MemSize;
-        "MC"    :: Bool;
-        "LM"    :: Bool;
-        "LG"    :: Bool;
-        "sign?" :: Bool;
-        "cap?"  :: Bool }.
-
-  Theorem sizeMemOpInfo: size MemOpInfo <= CapSz.
-  Proof.
-    simpl.
-    unfold MemSize, MemSizeSz, CapSz, Xlen, MemOpSz.
-    destruct procParams as [xlen xlen_vars].
-    destruct xlen_vars; subst; simpl; lia.
-  Qed.
-
-  Definition FullOutput :=
-    STRUCT_TYPE {
-        "wb?" :: Bool;
-        "cdTag" :: Bool;
-        "cdCap" :: Cap;
-        "cdVal" :: Data;
-        "taken?" :: Bool;
-        "pcMemAddr" :: Addr;
-        "changePcCap?" :: Bool;
-        "pcCap" :: Cap;
-        "changeIe?" :: Bool;
-        "newIe" :: Bool;
-        "exception?" :: Bool;
-        "exceptionCause" :: Data;
-        "exceptionValue" :: Addr;
-        "baseException?" :: Bool;
-        "pcCapException?" :: Bool;
-        "mem?" :: Bool;
-        "memCap?" :: Bool;
-        "memSize" :: MemSize;
-        "store?" :: Bool;
-        "ldSigned?" :: Bool;
-        "ldPerms" :: CapPerms;
-        "fenceI?" :: Bool;
-        "wbScr?" :: Bool;
-        "scrTag" :: Bool;
-        "scrCap" :: Cap;
-        "scrVal" :: Data;
-        "scrException?" :: Bool;
-        "wbCsr?" :: Bool;
-        "csrVal" :: Data }.
-
-  Section InstEntry.
-    Variable ik: Kind.
-    Record InstEntry :=
-      { instName       : string;
-        uniqId         : UniqId;
-        immEncoder     : list ImmEncoder;
-        spec           : forall ty, FullCap @# ty -> Inst @# ty ->
-                                    FullCapWithTag @# ty -> FullCapWithTag @# ty ->
-                                    FullCapWithTag @# ty -> Data @# ty -> ik ## ty;
-        instProperties : InstProperties;
-        goodInstEncode : isGoodInstEncode uniqId immEncoder instProperties;
-        immStart       : nat;
-        immEnd         : nat;
-        goodImmEncode  : getDisjointContiguous (concat (map immPos immEncoder)) = Some (immStart, immEnd)
-      }.
-
-    Record InstEntryFull := {
-        xlens : list nat;
-        extension: Extension;
-        instEntries: list InstEntry }.
-
-    Section Encoder.
-      Variable i: InstEntry.
-      Variable cs1 cs2 cd: word (snd rs1FixedField).
-      Variable csr: word (snd immField).
-      Variable immV: word Xlen.
-      Fixpoint encodeImmField (imms: list (nat * nat)) :=
-        match imms return word (fold_right (fun '(_, val) sum => sum + val) 0 imms) with
-        | nil => WO
-        | (start, width) :: xs => wcombine (encodeImmField xs) (extractWord immV start width)
-        end.
-
-      Definition encodeFullInstList :=
-        uniqId i ++
-          map (fun ie => existT _ (instPos ie, _) (encodeImmField (immPos ie))) (immEncoder i) ++
-          (if hasCs1 (instProperties i) then [existT _ rs1FixedField cs1] else []) ++
-          (if hasCs2 (instProperties i) then [existT _ rs2FixedField cs2] else []) ++
-          (if hasCd (instProperties i) then [existT _ rdFixedField cd] else []) ++
-          (if hasScr (instProperties i) then [existT _ rs2FixedField cs2] else []) ++
-          (if hasCsr (instProperties i) then [existT _ immField csr] else []).
-
-      Definition encodeInst := @truncLsb InstSz _ ((wordCombiner (2'b"11") (SigWordSort.sort encodeFullInstList))).
-    End Encoder.
-
-    Section Decoder.
-      Variable inst: word InstSz.
-      Fixpoint immDecoderHelp (instStart: nat) (ls: list (nat * nat)) : list FieldRange :=
-        match ls with
-        | nil => nil
-        | (immStart, width) :: xs => existT _ (immStart, width) (extractWord inst instStart width) ::
-                                       immDecoderHelp (instStart + width) xs
-        end.
-
-      Definition immDecoder (immEnc: ImmEncoder) :=
-        immDecoderHelp (instPos immEnc) (immPos immEnc).
-
-      Variable i: InstEntry.
-
-      Definition decodePartialImmList :=
-        SigWordSort.sort (concat (map immDecoder (immEncoder i))).
-
-      Definition decodeImm: word Xlen :=
-        match decodePartialImmList with
-        | nil => wzero Xlen
-        | existT (start, _) _ :: _ =>
-            let res := wordCombiner (wzero start) decodePartialImmList in
-            wconcat
-              (if (andb (signExt (instProperties i)) (weqb (get_msb res) WO~1))
-               then wones _
-               else wzero (Xlen - (fold_right (fun new sum => sum + snd (projT1 new)) start decodePartialImmList)))
-              res
-        end.
-    End Decoder.
-
-    Section DecoderExpr.
-      Variable ty: Kind -> Type.
-      Variable inst: Inst @# ty.
-      Fixpoint immDecIntervalHelp (instStart: nat) (ls: list (nat * nat)) : list (nat * (nat * nat)) :=
-        match ls with
-        | nil => nil
-        | (immStart, width) :: xs => (immStart, (instStart, width)) :: immDecIntervalHelp (instStart + width) xs
-        end.
-
-      Definition immDecInterval (immEnc: ImmEncoder) :=
-        immDecIntervalHelp (instPos immEnc) (immPos immEnc).
-
-      Variable i: InstEntry.
-
-      Definition decIntervals :=
-        SigTripleSort.sort (concat (map immDecInterval (immEncoder i))).
-
-      Definition decExprs := map (fun x =>
-                                    existT (fun x => Bit (snd x) @# ty)
-                                      (fst x, snd (snd x)) (extractBits inst (fst (snd x)) (snd (snd x))))
-                               decIntervals.
-
-      Definition decodeImmExpr :=
-        match decExprs with
-        | nil => Const ty (wzero Xlen)
-        | (existT (start, _) _) :: _ =>
-            let res := bitsCombiner (Const ty (wzero start)) decExprs in
-            if signExt (instProperties i)
-            then SignExtendTruncLsb Xlen res
-            else ZeroExtendTruncLsb Xlen res
-        end.
-    End DecoderExpr.
-  End InstEntry.
-
-  Record FuncEntryFull :=
-    { funcNameFull        : string;
-      localFuncInputFull  : Kind;
-      localFuncFull       : forall ty, localFuncInputFull @# ty -> FullOutput ## ty;
-      instsFull           : list (InstEntryFull localFuncInputFull) }.
-
-  Record FuncEntry :=
-    { funcName        : string;
-      localFuncInput  : Kind;
-      localFunc       : forall ty, localFuncInput @# ty -> FullOutput ## ty;
-      insts           : list (InstEntry localFuncInput) }.
-
-  Definition filterInsts k (ls: list (InstEntryFull k)) :=
-    fold_right (fun new rest =>
-                  (if (getBool (in_dec Nat.eq_dec Xlen (xlens new)) &&
-                         getBool (in_dec Extension_eq_dec (extension new) supportedExts))%bool
-                   then instEntries new
-                   else []) ++ rest) [] ls.
-  
-  Definition mkFuncEntry (fe : FuncEntryFull) :=
-    {|funcName := funcNameFull fe;
-      localFuncInput := localFuncInputFull fe;
-      localFunc := localFuncFull fe;
-      insts := filterInsts (instsFull fe)
-    |}.
-
-  Record ScrReg :=
-    { scrRegInfo    : RegInfo (snd rs2FixedField) FullCapWithTag;
-      isLegal       : forall ty, Data @# ty -> Bool @# ty;
-      legalize      : forall ty, Data @# ty -> Data @# ty }.
-
-  Record CsrReg :=
-    { csrRegInfo    : RegInfo (snd immField) Data;
-      isSystemCsr   : bool;
-      csrMask       : option (word Xlen) }.
-
-  Theorem XlenSXlenMinus1: Xlen = ((S (Xlen - 1)) * 1)%nat.
-  Proof.
-    destruct procParams as [xlen xlen_vars].
-    destruct xlen_vars; subst; simpl; lia.
-  Qed.
-
-  Section ReadArray.
-    Variable ty: Kind -> Type.
-    Variable addr: Addr @# ty.
-    Variable n: nat.
-    Variable arr: Array n (Bit 8) @# ty.
-    Local Open Scope kami_expr.
-    Definition readArrayConstSize (size: nat) :=
-      BuildArray (fun (i: Fin.t size) => arr@[addr + $(FinFun.Fin2Restrict.f2n i)]).
-  End ReadArray.
-End ParamDefinitions.
+Record CsrReg :=
+  { csrRegInfo    : RegInfo Imm12Sz;
+    isSystemCsr   : bool;
+    csrMask       : option (word Xlen) }.
