Cheriot/CheriotTypes.v
@@ -1,0 +1,348 @@
+Require Import Kami.AllNotations ProcKami.Cheriot.Lib.
+Require Import RecordUpdate.RecordUpdate.
+
+Definition compressed := false.
+
+Inductive Extension := Base | M.
+Definition supportedExts := [Base].
+
+Definition RegIdSz := 5.
+Definition NumRegs := Nat.pow 2 RegIdSz.
+Definition RegFixedIdSz := 5.
+
+Definition CapRSz := 1.
+Definition CapOTypeSz := 3.
+Definition CapPermSz := 6.
+Definition CapESz := 4.
+Definition CapBTSz := 9.
+
+Definition Xlen := 32.
+Definition AddrSz := Xlen.
+Definition Data := Bit Xlen.
+Definition Addr := Bit AddrSz.
+Definition LgAddrSz := Nat.log2_up AddrSz.
+
+Definition InstSz := 32.
+Definition CompInstSz := 16.
+
+Definition Imm12Sz := 12.
+Definition Imm20Sz := 20.
+Definition instSizeField := (0, 2).
+Definition opcodeField := (2, 5).
+Definition funct3Field := (12, 3).
+Definition funct7Field := (25, 7).
+Definition funct6Field := (26, 6).
+Definition immField := (20, Imm12Sz).
+Definition rs1Field := (15, RegIdSz).
+Definition rs2Field := (20, RegIdSz).
+Definition rdField := (7, RegIdSz).
+Definition rs1FixedField := (15, RegFixedIdSz).
+Definition rs2FixedField := (20, RegFixedIdSz).
+Definition rdFixedField := (7, RegFixedIdSz).
+Definition auiLuiField := (12, Imm20Sz).
+
+Definition imm12   := [(0, Imm12Sz)].
+Definition imm5    := [(0, 5)].
+Definition imm20_U := [(12, Imm20Sz)].
+Definition imm20_J := [(12, 8); (11, 1); (1, 10); (20, 1)].
+Definition imm6    := [(0, 6)].
+Definition imm7    := [(5, 7)].
+Definition imm5_B  := [(11, 1); (1, 4)].
+Definition imm7_B  := [(5, 6); (12, 1)].
+
+Definition ScrIdSz := 5.
+
+Definition CapException        := N.to_nat (hex "1c").
+Definition CapBoundsViolation  := 1.  (* Reg/PC *)
+Definition CapTagViolation     := 2.  (* Reg *)
+Definition CapSealViolation    := 3.  (* Reg *)
+Definition CapExecViolation    := 17. (* Reg *)
+Definition CapLdViolation      := 18. (* Reg *)
+Definition CapStViolation      := 19. (* Reg *)
+Definition CapStCapViolation   := 21. (* Reg *)
+Definition CapStLocalViolation := 22. (* Reg *)
+Definition CapSysRegViolation  := 24. (* PC *)
+Definition CapLdMisaligned     := 4.  (* Addr *)
+Definition CapStMisaligned     := 6.  (* Addr *)
+
+Definition InstMisaligned      := 0.  (* Addr *)
+Definition InstAccessFault     := 1.  (* Addr *)
+Definition InstPageFault       := 12. (* Addr *)
+Definition LoadAccessFault     := 5.  (* Addr *)
+Definition LoadPageFault       := 13. (* Addr *)
+Definition StoreAccessFault    := 7.  (* Addr *)
+Definition StorePageFault      := 15. (* Addr *)
+Definition TagAccessFault      := 24. (* Addr *)
+Definition TagPageFault        := 25. (* Addr *)
+Definition InstIllegal         := 2.  (* Inst *)
+Definition ECall               := 8.
+
+Section Fields.
+  Variable ty: Kind -> Type.
+  Variable inst: Bit InstSz @# ty.
+
+  Local Open Scope kami_expr.
+
+  Notation extractFieldFromInst span := (extractFieldExpr InstSz inst (fst span) (snd span)).
+
+  Definition instSize := extractFieldFromInst instSizeField.
+  Definition opcode := extractFieldFromInst opcodeField.
+  Definition funct3 := extractFieldFromInst funct3Field.
+  Definition funct7 := extractFieldFromInst funct7Field.
+  Definition funct6 := extractFieldFromInst funct6Field.
+  Definition rs1 := extractFieldFromInst rs1Field.
+  Definition rs2 := extractFieldFromInst rs2Field.
+  Definition rd := extractFieldFromInst rdField.
+  Definition rs1Fixed := extractFieldFromInst rs1FixedField.
+  Definition rs2Fixed := extractFieldFromInst rs2FixedField.
+  Definition rdFixed := extractFieldFromInst rdFixedField.
+
+  (* TODO: These should be derived from encoder/decoder *)
+  Definition imm := extractFieldFromInst immField.
+  Definition branchOffset := ({< extractFieldFromInst (31, 1),
+                                 extractFieldFromInst ( 7, 1),
+                                 extractFieldFromInst (25, 6),
+                                 extractFieldFromInst ( 8, 4), $$(WO~0) >}).
+  Definition jalOffset := ({< extractFieldFromInst (31,  1),
+                              extractFieldFromInst (12,  8),
+                              extractFieldFromInst (20,  1),
+                              extractFieldFromInst (21, 10), $$(WO~0) >}).
+  Definition auiLuiOffset := extractFieldFromInst auiLuiField.
+End Fields.
+
+Notation mtcc := 28%Z.
+Notation mtdc := 29%Z.
+Notation mscratchc := 30%Z.
+Notation mepcc := 31%Z.
+
+Notation mstatus := (Z.of_N (hex "300")).
+Notation mie := (Z.of_N (hex "304")).
+Notation mcause := (Z.of_N (hex "342")).
+Notation mtval := (Z.of_N (hex "343")).
+
+Definition Cap : Kind :=
+  (STRUCT_TYPE {
+       "R" :: Bit CapRSz;
+       "p" :: Bit CapPermSz;
+       "oType" :: Bit CapOTypeSz;
+       "E" :: Bit CapESz;
+       "T" :: Bit CapBTSz;
+       "B" :: Bit CapBTSz })%kami_expr.
+
+Definition CapSz := size Cap.
+
+Goal CapSz = Xlen.
+Proof.
+  reflexivity.
+Qed.
+
+Definition NumBanks := (Xlen + CapSz) / 8.
+
+Definition CapPerms :=
+  STRUCT_TYPE {
+      "U0" :: Bool;
+      "SE" :: Bool; (* Permit Seal *)
+      "US" :: Bool; (* Permit Unseal *)
+      "EX" :: Bool; (* Permit Execute *)
+      "SR" :: Bool; (* Permit system register access *)
+      "MC" :: Bool; (* Permit Load or Store of Caps *)
+      "LD" :: Bool; (* Permit Load *)
+      "SL" :: Bool; (* Permit Store of Local *)
+      "LM" :: Bool; (* Permit Mutability of loaded cap, i.e. allow store using the cap *)
+      "SD" :: Bool; (* Permit Store *)
+      "LG" :: Bool; (* Permit Store into Global of loaded cap *)
+      "GL" :: Bool }. (* Global *)
+
+Definition FullCapWithTag := STRUCT_TYPE { "tag" :: Bool ;
+                                           "cap" :: Cap ;
+                                           "val" :: Data }.
+
+Definition FullCap := STRUCT_TYPE { "cap" :: Cap ;
+                                    "val" :: Data }.
+
+Definition MaxExp := AddrSz - CapBTSz - 1.
+
+Section CapHelpers.
+  Variable ty: Kind -> Type.
+  Local Open Scope kami_expr.
+  Definition decodePerms (rawPerms: Array CapPermSz Bool @# ty) : CapPerms @# ty :=
+    (IF rawPerms ![4]
+     then (IF rawPerms ![3]
+           then (STRUCT {
+                     "U0" ::= $$false;
+                     "SE" ::= $$false;
+                     "US" ::= $$false;
+                     "EX" ::= $$false;
+                     "SR" ::= $$false;
+                     "MC" ::= $$true;
+                     "LD" ::= $$true;
+                     "SL" ::= rawPerms ![2];
+                     "LM" ::= rawPerms ![1];
+                     "SD" ::= $$true;
+                     "LG" ::= rawPerms ![0];
+                     "GL" ::= rawPerms ![5] })
+           else (IF rawPerms ![2]
+                 then (STRUCT {
+                           "U0" ::= $$false;
+                           "SE" ::= $$false;
+                           "US" ::= $$false;
+                           "EX" ::= $$false;
+                           "SR" ::= $$false;
+                           "MC" ::= $$true;
+                           "LD" ::= $$true;
+                           "SL" ::= $$false;
+                           "LM" ::= rawPerms ![1];
+                           "SD" ::= $$false;
+                           "LG" ::= rawPerms ![0];
+                           "GL" ::= rawPerms ![5] })
+                 else (IF !(rawPerms ![1]) && !(rawPerms ![0])
+                       then (STRUCT {
+                                 "U0" ::= $$false;
+                                 "SE" ::= $$false;
+                                 "US" ::= $$false;
+                                 "EX" ::= $$false;
+                                 "SR" ::= $$false;
+                                 "MC" ::= $$true;
+                                 "LD" ::= $$false;
+                                 "SL" ::= $$false;
+                                 "LM" ::= $$false;
+                                 "SD" ::= $$true;
+                                 "LG" ::= $$false;
+                                 "GL" ::= rawPerms ![5] })
+                       else (STRUCT {
+                                 "U0" ::= $$false;
+                                 "SE" ::= $$false;
+                                 "US" ::= $$false;
+                                 "EX" ::= $$false;
+                                 "SR" ::= $$false;
+                                 "MC" ::= $$false;
+                                 "LD" ::= rawPerms ![1];
+                                 "SL" ::= $$false;
+                                 "LM" ::= $$false;
+                                 "SD" ::= rawPerms ![0];
+                                 "LG" ::= $$false;
+                                 "GL" ::= rawPerms ![5] }))))
+     else (IF rawPerms ![3]
+           then (STRUCT {
+                     "U0" ::= $$false;
+                     "SE" ::= $$false;
+                     "US" ::= $$false;
+                     "EX" ::= $$true;
+                     "SR" ::= rawPerms ![2];
+                     "MC" ::= $$true;
+                     "LD" ::= $$true;
+                     "SL" ::= $$false;
+                     "LM" ::= rawPerms ![1];
+                     "SD" ::= $$false;
+                     "LG" ::= rawPerms ![0];
+                     "GL" ::= rawPerms ![5] })
+           else (STRUCT {
+                     "U0" ::= rawPerms ![2];
+                     "SE" ::= rawPerms ![1];
+                     "US" ::= rawPerms ![0];
+                     "EX" ::= $$false;
+                     "SR" ::= $$false;
+                     "MC" ::= $$false;
+                     "LD" ::= $$false;
+                     "SL" ::= $$false;
+                     "LM" ::= $$false;
+                     "SD" ::= $$false;
+                     "LG" ::= $$false;
+                     "GL" ::= rawPerms ![5] }))).
+
+  Definition encodePerms (perms: CapPerms @# ty) : Bit CapPermSz @# ty :=
+    {< pack (perms @% "GL"),
+      ( IF perms @% "EX" && perms @% "LD" && perms @% "MC"
+        then {< Const ty (2'b"01"), pack (perms @% "SR"), pack (perms @% "LM"), pack (perms @% "LG") >}
+        else (IF perms @% "LD" && perms @% "MC" && perms @% "SD"
+              then {< Const ty (2'b"11"), pack (perms @% "SL"), pack (perms @% "LM"), pack (perms @% "LG") >}
+              else (IF perms @% "LD" && perms @% "MC"
+                    then {< Const ty (3'b"101"), pack (perms @% "LM"), pack (perms @% "LG") >}
+                    else (IF perms @% "SD" && perms @% "MC"
+                          then Const ty (5'b"10000")
+                          else (IF perms @% "LD" || perms @% "SD"
+                                then {< Const ty (3'b"100"), pack (perms @% "LD"), pack (perms @% "SD") >}
+                                else {< Const ty (2'b"00"), pack (perms @% "U0"), pack (perms @% "SE"),
+                                   pack (perms @% "US") >})))))%kami_expr >}.
+
+  Definition getCapExpFromE (E: Bit CapESz @# ty) : Bit LgAddrSz @# ty :=
+    ITE (E == Const ty (wones _)) $MaxExp (ZeroExtend _ E).
+  
+  Definition getCapEFromExp (exp: Bit LgAddrSz @# ty) : Bit CapESz @# ty :=
+    ITE (exp >= $(Nat.pow 2 CapESz - 1)) $$(wones CapESz) (UniBit (TruncLsb CapESz _) exp).
+
+  Definition getCapOTypeFromIe ie: Bit CapOTypeSz @# ty := ITE ie $2 $3.
+
+  Definition isCapSealAddr (addr: Addr @# ty) isExec := ITE isExec
+                                                          (((addr >= $1) && (addr <= $3)) || addr == $6 || addr == $7)
+                                                          ((addr >= $9) && (addr <= $15)).
+
+  Definition getCapBounds (base: Bit AddrSz @# ty) (length: Bit AddrSz @# ty) :=
+    ( LETC top : Bit (AddrSz + 1) <- ZeroExtend 1 base + ZeroExtend 1 length;
+      LETC expInit : Bit LgAddrSz <-
+                       $(AddrSz - CapBTSz) - (countLeadingZeros _ (UniBit (TruncMsb (AddrSz - CapBTSz) _) length));
+      LETC isInitSatExpInitSat : Pair Bool (Bit LgAddrSz) <-
+                                   ITE (#expInit > $(Nat.pow 2 CapESz - 2)) (STRUCT { "fst" ::= $$true;
+                                                                                      "snd" ::= $MaxExp })
+                                     (STRUCT { "fst" ::= $$false; "snd" ::= #expInit });
+      LETC isInitSat <- #isInitSatExpInitSat @% "fst";
+      LETC expInitSat <- #isInitSatExpInitSat @% "snd";
+      LETC lostTopInit <- isNotZero (#top << ($AddrSz - #expInitSat));
+      LETC lengthShifted <- UniBit (TruncLsb CapBTSz _) (length >> #expInitSat);
+      LETC lengthShiftedAllOnes <- isAllOnes #lengthShifted;
+      LETC exp : Bit LgAddrSz <- ITE (#lostTopInit && #lengthShiftedAllOnes && !#isInitSat)
+                                   (#expInitSat + $1) (#expInitSat);
+      LETC B <- UniBit (TruncLsb CapBTSz _) (base >> #exp);
+      LETC lostTop <- isNotZero (#top << ($AddrSz - #exp));
+      LETC TInit <- UniBit (TruncLsb CapBTSz _) (#top >> #exp);
+      LETC T <- ITE #lostTop (#TInit + $1) #TInit;
+      LETC lostBase <- isNotZero (base << ($AddrSz - #exp));
+      RetE (STRUCT {
+                "B" ::= #B;
+                "T" ::= #T;
+                "exp" ::= #exp;
+                "exact?" ::= (#lostBase || #lostTop) } : STRUCT_TYPE { "B" :: Bit CapBTSz;
+                                                                       "T" :: Bit CapBTSz;
+                                                                       "exp" :: Bit LgAddrSz;
+                                                                       "exact?" :: Bool } @# ty)).
+
+  Definition getBaseTop (B T: Bit CapBTSz @# ty) (E: Bit CapESz @# ty) (addr: Addr @# ty) :=
+    ( LETC exp <- getCapExpFromE E;
+      LETC aMidTop <- addr >> #exp;
+      LETC aMid <- UniBit (TruncLsb CapBTSz (AddrSz - CapBTSz)) #aMidTop;
+      LETC aTop <- UniBit (TruncMsb CapBTSz (AddrSz - CapBTSz)) #aMidTop;
+      LETC aHi <- ITE (#aMid < B) $1 $0;
+      LETC tHi <- ITE (T < B) $1 $0;
+      LETC aTopBase <- #aTop - #aHi;
+      LETC aTopTop <- (ZeroExtend 1 #aTopBase) + #tHi;
+      LETC base: Addr <- ZeroExtend _ ({< #aTopBase, B >}) << #exp;
+      LETC top: Bit (AddrSz + 1) <- ZeroExtend _ ({< #aTopTop, T >}) << #exp;
+      RetE (STRUCT {
+                "base" ::= #base;
+                "top" ::= #top;
+                "aTopBase" ::= #aTopBase } : (STRUCT_TYPE { "base" :: Bit AddrSz ;
+                                                            "top"  :: Bit (AddrSz + 1) ;
+                                                            "aTopBase" :: Bit (AddrSz - CapBTSz) }) @# ty) ).
+
+  Section GivenCap.
+    Variable cap: Cap @# ty.
+    
+    Definition isCapSealed := isNotZero (cap @% "oType").
+    Definition isCapSentry := (cap @% "oType" >= $1) && (cap @% "oType" <= $3).
+    Definition isCapIeSentry := (cap @% "oType" == $2).
+    Definition isCapIdSentry := (cap @% "oType" == $3).
+
+    Definition sealCap (val: Bit CapOTypeSz @# ty) := cap @%[ "oType" <- val ] : Cap @# ty.
+    Definition unsealCap := cap @%[ "oType" <- Const ty (wzero CapOTypeSz) ] : Cap @# ty.
+
+    Definition getCapPerms : CapPerms @# ty := decodePerms (unpack (Array CapPermSz Bool) (cap @% "p")).
+  End GivenCap.
+
+  Definition getCapBaseTop (cap: FullCap @# ty) :=
+    getBaseTop (cap @% "cap" @% "B") (cap @% "cap" @% "T") (cap @% "cap" @% "E") (cap @% "val").
+  
+  Definition representableFnCap (cap: FullCap @# ty) (addr: Addr @# ty) : Bool ## ty :=
+    ( LETE baseTop <- getBaseTop (cap @% "cap" @% "B") (cap @% "cap" @% "T") (cap @% "cap" @% "E") (cap @% "val");
+      LETE baseTop2 <- getBaseTop (cap @% "cap" @% "B") (cap @% "cap" @% "T") (cap @% "cap" @% "E") addr;
+      RetE ((#baseTop @% "aTopBase") == (#baseTop2 @% "aTopBase")) ).
+End CapHelpers.
