Cheriot/CoreConfig.v
@@ -1,313 +1,12 @@
 Require Import Kami.AllNotations.
 Require Import ProcKami.Cheriot.Lib ProcKami.Cheriot.Types ProcKami.Cheriot.InstSpec ProcKami.Cheriot.SpecRun.
 
-Definition CapStruct : Kind :=
-  (STRUCT_TYPE {
-       "R" :: Bit 1;
-       "p" :: Bit 6;
-       "oType" :: Bit 3;
-       "E" :: Bit 4;
-       "B" :: Bit 9;
-       "T" :: Bit 9 })%kami_expr.
-
-Section CapHelpers.
-  Local Notation AddrSz := 32.
-  Section ty.
-    Variable ty: Kind -> Type.
-    Local Open Scope kami_expr.
-    Definition decodePerms (rawPerms: Array 6 Bool @# ty) : CapPerms @# ty :=
-      (IF rawPerms ![4]
-       then (IF rawPerms ![3]
-             then (STRUCT {
-                       "U0" ::= $$false;
-                       "SE" ::= $$false;
-                       "US" ::= $$false;
-                       "EX" ::= $$false;
-                       "SR" ::= $$false;
-                       "MC" ::= $$true;
-                       "LD" ::= $$true;
-                       "SL" ::= rawPerms ![2];
-                       "LM" ::= rawPerms ![1];
-                       "SD" ::= $$true;
-                       "LG" ::= rawPerms ![0];
-                       "GL" ::= rawPerms ![5] })
-             else (IF rawPerms ![2]
-                   then (STRUCT {
-                             "U0" ::= $$false;
-                             "SE" ::= $$false;
-                             "US" ::= $$false;
-                             "EX" ::= $$false;
-                             "SR" ::= $$false;
-                             "MC" ::= $$true;
-                             "LD" ::= $$true;
-                             "SL" ::= $$false;
-                             "LM" ::= rawPerms ![1];
-                             "SD" ::= $$false;
-                             "LG" ::= rawPerms ![0];
-                             "GL" ::= rawPerms ![5] })
-                   else (IF !(rawPerms ![1]) && !(rawPerms ![0])
-                         then (STRUCT {
-                                   "U0" ::= $$false;
-                                   "SE" ::= $$false;
-                                   "US" ::= $$false;
-                                   "EX" ::= $$false;
-                                   "SR" ::= $$false;
-                                   "MC" ::= $$true;
-                                   "LD" ::= $$false;
-                                   "SL" ::= $$false;
-                                   "LM" ::= $$false;
-                                   "SD" ::= $$true;
-                                   "LG" ::= $$false;
-                                   "GL" ::= rawPerms ![5] })
-                         else (STRUCT {
-                                   "U0" ::= $$false;
-                                   "SE" ::= $$false;
-                                   "US" ::= $$false;
-                                   "EX" ::= $$false;
-                                   "SR" ::= $$false;
-                                   "MC" ::= $$false;
-                                   "LD" ::= rawPerms ![1];
-                                   "SL" ::= $$false;
-                                   "LM" ::= $$false;
-                                   "SD" ::= rawPerms ![0];
-                                   "LG" ::= $$false;
-                                   "GL" ::= rawPerms ![5] }))))
-       else (IF rawPerms ![3]
-             then (STRUCT {
-                       "U0" ::= $$false;
-                       "SE" ::= $$false;
-                       "US" ::= $$false;
-                       "EX" ::= $$true;
-                       "SR" ::= rawPerms ![2];
-                       "MC" ::= $$true;
-                       "LD" ::= $$true;
-                       "SL" ::= $$false;
-                       "LM" ::= rawPerms ![1];
-                       "SD" ::= $$false;
-                       "LG" ::= rawPerms ![0];
-                       "GL" ::= rawPerms ![5] })
-             else (STRUCT {
-                       "U0" ::= rawPerms ![2];
-                       "SE" ::= rawPerms ![1];
-                       "US" ::= rawPerms ![0];
-                       "EX" ::= $$false;
-                       "SR" ::= $$false;
-                       "MC" ::= $$false;
-                       "LD" ::= $$false;
-                       "SL" ::= $$false;
-                       "LM" ::= $$false;
-                       "SD" ::= $$false;
-                       "LG" ::= $$false;
-                       "GL" ::= rawPerms ![5] }))).
-    
-    Definition encodePerms (perms: CapPerms @# ty) : Bit 6 @# ty :=
-      {< pack (perms @% "GL"),
-        ( IF perms @% "EX" && perms @% "LD" && perms @% "MC"
-          then {< Const ty (2'b"01"), pack (perms @% "SR"), pack (perms @% "LM"), pack (perms @% "LG") >}
-          else (IF perms @% "LD" && perms @% "MC" && perms @% "SD"
-                then {< Const ty (2'b"11"), pack (perms @% "SL"), pack (perms @% "LM"), pack (perms @% "LG") >}
-                else (IF perms @% "LD" && perms @% "MC"
-                      then {< Const ty (3'b"101"), pack (perms @% "LM"), pack (perms @% "LG") >}
-                      else (IF perms @% "SD" && perms @% "MC"
-                            then Const ty (5'b"10000")
-                            else (IF perms @% "LD" || perms @% "SD"
-                                  then {< Const ty (3'b"100"), pack (perms @% "LD"), pack (perms @% "SD") >}
-                                  else {< Const ty (2'b"00"), pack (perms @% "U0"), pack (perms @% "SE"), pack (perms @% "US") >})))))%kami_expr >}.
-    
-    Definition capExpFromE (E: Bit 4 @# ty) : Bit (Nat.log2_up AddrSz) @# ty :=  ITE (E == Const ty (wones _)) $24 (ZeroExtendTruncLsb _ E).
-    
-    Definition capBaseTop (cap: Bit (size CapStruct) @# ty) (addr: Bit AddrSz @# ty) :=
-      ( LETC B <- (unpack CapStruct cap) @% "B";
-        LETC T <- (unpack CapStruct cap) @% "T";
-        LETC E <- (unpack CapStruct cap) @% "E";
-        LETC exp <- capExpFromE #E;
-        LETC aMidTop <- addr >> #exp;
-        LETC aMid <- UniBit (TruncLsb 9 (AddrSz - 9)) #aMidTop;
-        LETC aTop <- UniBit (TruncMsb 9 (AddrSz - 9)) #aMidTop;
-        LETC aHi <- ITE (#aMid < #B) $1 $0;
-        LETC tHi <- ITE (#T < #B) $1 $0;
-        LETC aTopBase <- #aTop - #aHi;
-        LETC aTopTop <- (ZeroExtend 1 #aTopBase) + #tHi;
-        LETC base <- ZeroExtendTruncLsb AddrSz ({< #aTopBase, #B >}) << #exp;
-        LETC top <- ZeroExtendTruncLsb (AddrSz + 1) ({< #aTopTop, #T >}) << #exp;
-        RetE (STRUCT {
-                  "base" ::= #base;
-                  "top" ::= #top;
-                  "aTopBase" ::= #aTopBase } : (STRUCT_TYPE { "base" :: Bit AddrSz ;
-                                                              "top"  :: Bit (AddrSz + 1) ;
-                                                              "aTopBase" :: Bit (AddrSz - 9) }) @# ty) ).
-    
-    Definition capBounds (base: Bit AddrSz @# ty) (length: Bit AddrSz @# ty) :=
-      ( LETC top : Bit (AddrSz + 1) <- ZeroExtend 1 base + ZeroExtend 1 length;
-        LETC expInit : Bit (Nat.log2_up AddrSz) <- $23 - (countLeadingZeros _ (ZeroExtendTruncMsb 23 length));
-        LETC isInitSatExpInitSat : Pair Bool (Bit (Nat.log2_up AddrSz)) <-
-                                     ITE (#expInit > $14) (STRUCT { "fst" ::= $$true; "snd" ::= $$(wones 5) })
-                                       (STRUCT { "fst" ::= $$false; "snd" ::= #expInit });
-        LETC isInitSat <- #isInitSatExpInitSat @% "fst";
-        LETC expInitSat <- #isInitSatExpInitSat @% "snd";
-        LETC lostTopInit <- isNotZero (#top << ($AddrSz - #expInitSat));
-        LETC lengthShifted <- ZeroExtendTruncLsb 9 (length >> #expInitSat);
-        LETC lengthShiftedAllOnes <- isAllOnes #lengthShifted;
-        LETC exp : Bit (Nat.log2_up AddrSz) <- ITE (#lostTopInit && #lengthShiftedAllOnes && !#isInitSat)
-                                                 (#expInitSat + $1) (#expInitSat);
-        LETC B <- ZeroExtendTruncLsb 9 (base >> #exp);
-        LETC lostTop <- isNotZero (#top << ($AddrSz - #exp));
-        LETC TInit <- ZeroExtendTruncLsb 9 (#top >> #exp);
-        LETC T <- ITE #lostTop (#TInit + $1) #TInit;
-        LETC lostBase <- isNotZero (base << ($AddrSz - #exp));
-        RetE (STRUCT {
-                  "B" ::= #B;
-                  "T" ::= #T;
-                  "exp" ::= #exp;
-                  "exact?" ::= (#lostBase || #lostTop) } : STRUCT_TYPE { "B" :: Bit 9;
-                                                                         "T" :: Bit 9;
-                                                                         "exp" :: Bit (Nat.log2_up AddrSz);
-                                                                         "exact?" :: Bool } @# ty)).
-
-    Definition capPerms cap :=
-      (RetE decodePerms (unpack (Array 6 Bool) ((unpack (ty := ty) CapStruct cap) @% "p"))).
-  End ty.
-  
-  Definition capAccessorsInit : CapAccessors _ _ :=
-    {|getCapR ty cap := (unpack CapStruct cap) @% "R";
-      setCapR ty val cap := pack ((unpack CapStruct cap) @%[ "R" <- val]);
-      getCapP ty cap := (unpack CapStruct cap) @% "p";
-      setCapP ty val cap := pack ((unpack CapStruct cap) @%[ "p" <- val]);
-      getCapOType ty cap := (unpack CapStruct cap) @% "oType";
-      setCapOType ty val cap := pack ((unpack CapStruct cap) @%[ "oType" <- val]);
-      getCapE ty cap := (unpack CapStruct cap) @% "E";
-      setCapE ty val cap := pack ((unpack CapStruct cap) @%[ "E" <- val]);
-      getCapB ty cap := (unpack CapStruct cap) @% "B";
-      setCapB ty val cap := pack ((unpack CapStruct cap) @%[ "B" <- val]);
-      getCapT ty cap := (unpack CapStruct cap) @% "T";
-      setCapT ty val cap := pack ((unpack CapStruct cap) @%[ "T" <- val]);
-      getCapEFromExp ty exp := ITE (exp >= Const ty (_ 'h"e")) $$(4'h"f") (ZeroExtendTruncLsb _ exp);
-      getCapExpFromE ty E := capExpFromE E;
-      isSealed t cap := (unpack CapStruct cap) @% "oType" != $0;
-      isSentry t cap := let oType := (unpack CapStruct cap) @% "oType" in (oType <= $3) && (oType >= $1);
-      isIeSentry t cap := (unpack CapStruct cap) @% "oType" == $2;
-      isIdSentry t cap := (unpack CapStruct cap) @% "oType" == $3;
-      getOTypeFromIe ty ie := ITE ie $2 $3;
-      seal ty val cap := pack ((unpack CapStruct cap) @%[ "oType" <- val]);
-      unseal ty cap := pack ((unpack CapStruct cap) @%[ "oType" <- $$(natToWord 3 0)]);
-      isSealAddr ty addr isExec := ITE isExec
-                                     (((addr >= $1) && (addr <= $3)) || addr == $6 || addr == $7)
-                                     ((addr >= $9) && (addr <= $15));
-      getCapPerms ty cap := capPerms cap;
-      setCapPerms ty perms cap :=
-        ( LETC arr : Bit 6 <- encodePerms perms;
-          RetE (pack ((unpack CapStruct cap) @%[ "p" <- pack #arr ])) );
-      getCapBaseTop ty cap addr := capBaseTop cap addr;
-      getCapBounds ty base length := capBounds base length;
-    |}%kami_expr.
-
-  Definition ExecRootCapInit := evalExpr (@pack _ CapStruct
-                                            (STRUCT {
-                                                 "R" ::= Const _ (wzero _);
-                                                 "p" ::= Const _ ('b"101111");
-                                                 "oType" ::= Const _ (wzero _);
-                                                 "E" ::= Const _ (wones _);
-                                                 "B" ::= Const _ (wzero _);
-                                                 "T" ::= Const _ (_ 'h"100") })%kami_expr).
-
-  Definition DataRootCapInit := evalExpr (@pack _ CapStruct
-                                            ( STRUCT {
-                                                  "R" ::= Const _ (wzero _);
-                                                  "p" ::= Const _ ('b"111111");
-                                                  "oType" ::= Const _ (wzero _);
-                                                  "E" ::= Const _ (wones _);
-                                                  "B" ::= Const _ (wzero _);
-                                                  "T" ::= Const _ (_ 'h"100") })%kami_expr).
-
-  Definition SealRootCapInit := evalExpr (@pack _ CapStruct
-                                            (STRUCT {
-                                                 "R" ::= Const _ (wzero _);
-                                                 "p" ::= Const _ ('b"100111");
-                                                 "oType" ::= Const _ (wzero _);
-                                                 "E" ::= Const _ (wones _);
-                                                 "B" ::= Const _ (wzero _);
-                                                 "T" ::= Const _ (_ 'h"100") })%kami_expr).
-End CapHelpers.
-
-Definition FullCapWithTagKind := STRUCT_TYPE { "tag" :: Bool;
-                                               "cap" :: Bit 32;
-                                               "val" :: Bit 32 }.
-
-Class CoreConfigParams := {
-    prefix : string;
-    LgNumMemBytesVal: nat;
-    memInitVal: Fin.t (Nat.pow 2 LgNumMemBytesVal * 8) -> word 8;
-    regsInitVal: Fin.t 32 -> type FullCapWithTagKind;
-    pcCapInitVal: word 32;
-    pcCapValidThm: PcCapValid capAccessorsInit pcCapInitVal;
-    pcValInitVal: word 32;
-    pcValValidThm: truncLsb pcValInitVal = ZToWord 2 0;
-    mtccValInit: word 30;
-    mtdcValInit: word 30;
-    hasTrapVal: bool }.
-
 Section Prefix.
   Context `{coreConfigParams: CoreConfigParams}.
-  Lemma pccValidThm: PccValid capAccessorsInit pcCapInitVal pcValInitVal false.
-  Proof.
-    destruct coreConfigParams.
-    constructor; try intro; auto.
-  Qed.
+  Instance memParamsInst: MemParams := memParams.
 
-  Local Notation "@^ x" := (prefix ++ "_" ++ x)%string (at level 0).
-  Local Notation stringify x n := (prefix ++ "_" ++ (x ++ "_" ++ natToHexStr n)%string)%string.
-
-  Definition createMemRFParam (n: nat) : MemBankInit :=
-    {|instRqName := stringify "instRq" n;
-      loadRqName := stringify "loadRq" n;
-      storeRqName := stringify "storeRq" n;
-      memArrayName := stringify "memArray" n;
-      memRfString := stringify "memArrayFile" n |}.
-
-  Instance procParams : ProcParams :=
-    {|Xlen := 32;
-      xlenIs32_or_64 := or_introl eq_refl;
-      capAccessors := capAccessorsInit;
-      pccValid := pccValidThm;
-      ExecRootCap := ExecRootCapInit;
-      DataRootCap := DataRootCapInit;
-      SealRootCap := SealRootCapInit;
-      MtccVal := wcombine mtccValInit (wzero 2);
-      MtdcVal := wcombine mtdcValInit (wzero 2);
-      IeInit := false;
-      MeieInit := false;
-      MtieInit := false;
-      MsieInit := false;
-      supportedExts := [Base];
-      extsHasBase := or_introl eq_refl;
-      RegIdSz := 5;
-      regIdSzIs4_or5 := or_intror eq_refl;
-      memBankInits := map createMemRFParam (zeroToN 8);
-      lengthMemBankInits := eq_refl;
-      isMemAscii := false;
-      isMemRfArg := true;
-      memInit := memInitVal;
-      procName := prefix;
-      pcCapReg := @^"pcCap";
-      pcValReg := @^"pcVal";
-      prevPcCapReg := @^"prevPcCap";
-      prevPcValReg := @^"prevPcVal";
-      justFenceIReg := @^"justFenceIReg";
-      startFenceIReg := @^"startFenceIReg";
-      reqJustFenceIReg := @^"reqJustFenceIReg";
-      tagRead := @^"tagRead";
-      tagWrite := @^"tagWrite";
-      tagArray := @^"tagArray";
-      memArray := @^"memArray";
-      regsRead1 := @^"regsRead1";
-      regsRead2 := @^"regsRead2";
-      regsWrite := @^"regsWrite";
-      regsArray := @^"regsArray";
-      isRegsAscii := false;
-      isRegsRfArg := true;
-      regsRfString := @^"regsArrayFile";
-      regsInit := convConstArrayToFunConst regsInitVal;
-      hasTrap := hasTrapVal |}.
+  Local Notation "@^ x" := (procName ++ "_" ++ x)%string (at level 0).
+  Local Open Scope kami_expr.
 
   Definition getInstEntrySpec (fe: FuncEntry) : list (InstEntry FullOutput) :=
     map (fun ie => {|instName := instName ie;
@@ -328,14 +27,33 @@ Section Prefix.
       map (fun ie ty => specDecExecRule ty scrList csrList ie) specInstEntries.
 
   Definition specRegs : list RegInitT :=
-    (pcCapReg, existT _ (SyntaxKind (Bit CapSz)) (Some (SyntaxConst pcCapInitVal))) ::
-      (pcValReg, existT _ (SyntaxKind Addr) (Some (SyntaxConst pcValInitVal))) ::
-      (prevPcCapReg, existT _ (SyntaxKind (Bit CapSz)) (Some (SyntaxConst $0))) ::
-      (prevPcValReg, existT _ (SyntaxKind Addr) (Some (SyntaxConst $0))) ::
-      (regsArray, existT _ _ (Some (SyntaxConst (@convTypeToConst (Array 32 FullCapWithTagKind) regsInitVal)))) ::
-      (memArray, existT _ _ (Some (SyntaxConst (@convTypeToConst (Array (NumMemBytes * NumBanks) (Bit 8))
-                                                  memInitVal)))) ::
-      (tagArray, existT _ _ (Some (SyntaxConst (ConstArray (fun (i: Fin.t NumMemBytes) => false))))) ::
-      (map (fun x => (regName (scrRegInfo x), existT _ _ (regInit (scrRegInfo x)))) scrList) ++
-      (map (fun x => (regName (csrRegInfo x), existT _ _ (regInit (csrRegInfo x)))) csrList).
+    (@^pcCapReg, existT _ (SyntaxKind Cap) (Some (SyntaxConst (convTypeToConst pcCapInit)))) ::
+      (@^pcValReg, existT _ (SyntaxKind Addr) (Some (SyntaxConst (wcombine pcValInit (wzero 2))))) ::
+      (@^regsArray, existT _ _ (Some (SyntaxConst (@convTypeToConst (Array 32 FullCapWithTag) regsInit)))) ::
+      (@^memArray, existT _ _ (Some (SyntaxConst (@convTypeToConst (Array (NumMemBytes * NumBanks) (Bit 8))
+                                                    memInit)))) ::
+      (@^tagArray, existT _ _ (Some (SyntaxConst (ConstArray (fun (i: Fin.t NumMemBytes) => false))))) ::
+      (@^mtccReg,
+        existT _ _ (Some (SyntaxConst
+                            (convTypeToConst
+                               (evalExpr (STRUCT { "tag" ::= Const type true;
+                                                   "cap" ::= ExecRootCapExpr type;
+                                                   "val" ::= Const _ (wcombine mtccValInit (wzero 2))})))))) ::
+      (@^mtdcReg,
+        existT _ _ (Some (SyntaxConst
+                            (convTypeToConst
+                               (evalExpr (STRUCT { "tag" ::= Const type true;
+                                                   "cap" ::= DataRootCapExpr type;
+                                                   "val" ::= Const _ (wcombine mtdcValInit (wzero 2))})))))) ::
+      (@^mScratchCReg,
+        existT _ _ (Some (SyntaxConst
+                            (convTypeToConst
+                               (evalExpr (STRUCT { "tag" ::= Const type true;
+                                                   "cap" ::= SealRootCapExpr type;
+                                                   "val" ::= Const _ (wzero Xlen)})))))) ::
+      (@^mepccReg, existT _ _ (Some (SyntaxConst (getDefaultConst FullCapWithTag)))) ::
+      (@^mStatusReg, existT _ (SyntaxKind Data) (Some (SyntaxConst (wzero Xlen)))) ::
+      (@^mieReg, existT _ (SyntaxKind Data) (Some (SyntaxConst (wzero Xlen)))) ::
+      (@^mCauseReg, existT _ (SyntaxKind Data) None) ::
+      (@^mtValReg, existT _ (SyntaxKind Data) None) :: nil.
 End Prefix.
