Cheriot/MemSpec.v
@@ -1,12 +1,15 @@
 Require Import Kami.AllNotations ProcKami.Cheriot.Lib ProcKami.Cheriot.Types.
 
 Section MemSpec.
-  Context `{procParams: ProcParams}.
+  Variable procName: string.
+  Context `{memParams: MemParams}.
   
   Section ty.
     Variable ty: Kind -> Type.
     Local Open Scope kami_expr.
     Local Open Scope kami_action.
+
+    Local Notation "@^ x" := (procName ++ "_" ++ x)%string (at level 0).
 
     Section LoadStore.
       Variable pred: Bool @# ty.
@@ -17,52 +20,44 @@ Section MemSpec.
       Variable data: FullCapWithTag @# ty.
       
       Local Ltac dischargeDiv8 :=
-        unfold NumBanks, FullCap, Cap, CapSz, Data;
-        let H := fresh in
-        destruct (xlenIs32_or_64) as [H | H]; rewrite H; auto.
+        unfold NumBanks, FullCap, Cap, CapSz, Data; auto.
 
-      Definition loadReqSpec: ActionT ty FullCapWithTag.
-        refine
-          ( Read memArr : Array NumMemBytes (Bit 8) <- memArray;
-            LET ldBytes <- readArrayConstSize addr #memArr NumBanks;
-            LET ldSignVal <- (IF signed
-                              then TruncToDynamicSizeArraySigned #ldBytes size
-                              else TruncToDynamicSizeArrayUnsigned #ldBytes size);
-            LET ldVal <- unpack FullCap (castBits _ (pack #ldSignVal));
-            Read tags: Array NumMemBytes Bool <- tagArray;
-            LET tagIdx <- ZeroExtendTruncLsb (Nat.log2_up NumMemBytes)
-                            (ZeroExtendTruncMsb (Xlen - Nat.log2_up NumBanks) addr);
-            LET tag <- ITE isCap (#tags@[#tagIdx]) $$false;
-            Ret (STRUCT {
-                     "tag" ::= #tag;
-                     "cap" ::= #ldVal @% "cap";
-                     "val" ::= #ldVal @% "val" } : FullCapWithTag @# ty)).
-        abstract dischargeDiv8.
-      Defined.
+      Definition loadReqSpec: ActionT ty FullCapWithTag :=
+        ( Read memArr : Array NumMemBytes (Bit 8) <- @^memArray;
+          LET ldBytes <- readArrayConstSize addr #memArr NumBanks;
+          LET ldSignVal <- (IF signed
+                            then TruncToDynamicSizeArraySigned #ldBytes size
+                            else TruncToDynamicSizeArrayUnsigned #ldBytes size);
+          LET ldVal <- unpack FullCap (pack #ldSignVal);
+          Read tags: Array NumMemBytes Bool <- @^tagArray;
+          LET tagIdx <- ZeroExtendTruncLsb (Nat.log2_up NumMemBytes)
+                          (ZeroExtendTruncMsb (Xlen - Nat.log2_up NumBanks) addr);
+          LET tag <- ITE isCap (#tags@[#tagIdx]) $$false;
+          Ret (STRUCT {
+                   "tag" ::= #tag;
+                   "cap" ::= #ldVal @% "cap";
+                   "val" ::= #ldVal @% "val" } : FullCapWithTag @# ty)).
 
-      Definition storeReqSpec: ActionT ty Void.
-        refine
-          ( Read memArr : Array NumMemBytes (Bit 8) <- memArray;
-            LET idxLsb <- ZeroExtendTruncLsb (Nat.log2_up NumBanks) addr;
-            LET straddle <- ZeroExtend 1 #idxLsb + size <= $NumBanks;
-            LET tagIdx <- ZeroExtendTruncLsb (Nat.log2_up NumMemBytes)
-                            (ZeroExtendTruncMsb (Xlen - Nat.log2_up NumBanks) addr);
-            Read tags: Array NumMemBytes Bool <- tagArray;
-            LET updTag <- #tags@[ #tagIdx <- ITE isCap (data @% "tag") $$false];
-            (* #straddle implies !#isCap *)
-            LET updTagPlus1 <- #updTag@[ #tagIdx + $1 <- ITE #straddle $$false (#updTag@[#tagIdx + $1])];
-            LET stCapVal <- {< (data @% "cap"), (data @% "val") >};
-            LET stBytes <- unpack (Array NumBanks (Bit 8)) (castBits _ #stCapVal);
-            LET stArr <-
-              fold_left (fun newArr i => newArr @[addr + $i <- ITE ($i < size)
-                                                                 (#stBytes@[$$(natToWord (Nat.log2_up NumBanks) i)])
-                                                                 (newArr@[addr + $i])])
-                (seq 0 NumBanks) #memArr;
-            WriteIf pred Then memArray: Array NumMemBytes (Bit 8) <- #stArr;
-            WriteIf pred Then tagArray: Array NumMemBytes Bool <- #updTagPlus1;
-            Retv ).
-        abstract dischargeDiv8.
-      Defined.
+      Definition storeReqSpec: ActionT ty Void :=
+        ( Read memArr : Array NumMemBytes (Bit 8) <- @^memArray;
+          LET idxLsb <- ZeroExtendTruncLsb (Nat.log2_up NumBanks) addr;
+          LET straddle <- ZeroExtend 1 #idxLsb + size <= $NumBanks;
+          LET tagIdx <- ZeroExtendTruncLsb (Nat.log2_up NumMemBytes)
+                          (ZeroExtendTruncMsb (Xlen - Nat.log2_up NumBanks) addr);
+          Read tags: Array NumMemBytes Bool <- @^tagArray;
+          LET updTag <- #tags@[ #tagIdx <- ITE isCap (data @% "tag") $$false];
+          (* #straddle implies !#isCap *)
+          LET updTagPlus1 <- #updTag@[ #tagIdx + $1 <- ITE #straddle $$false (#updTag@[#tagIdx + $1])];
+          LET stCapVal <- {< pack (data @% "cap"), (data @% "val") >};
+          LET stBytes <- unpack (Array NumBanks (Bit 8)) #stCapVal;
+          LET stArr <-
+            fold_left (fun newArr i => newArr @[addr + $i <- ITE ($i < size)
+                                                               (#stBytes@[$$(natToWord (Nat.log2_up NumBanks) i)])
+                                                               (newArr@[addr + $i])])
+              (seq 0 NumBanks) #memArr;
+          WriteIf pred Then @^memArray: Array NumMemBytes (Bit 8) <- #stArr;
+          WriteIf pred Then @^tagArray: Array NumMemBytes Bool <- #updTagPlus1;
+          Retv ).
     End LoadStore.
   End ty.
 End MemSpec.
