Cheriot/SpecIsolation.v
@@ -3,25 +3,27 @@ Require Import ProcKami.Cheriot.Lib ProcKami.Cheriot.Types ProcKami.Cheriot.Core
 
 Section InBoundsTy.
   Variable ty: Kind -> Type.
-  Variable x inCap inVal: Bit 32 @# ty.
+  Variable x : Bit 32 @# ty.
+  Variable inCap: Cap @# ty.
+  Variable inVal: Bit 32 @# ty.
 
   Local Open Scope kami_expr.
 
-  Let inRange := capBaseTop inCap inVal.
+  Let inRange := getCapBaseTop (STRUCT { "cap" ::= inCap; "val" ::= inVal }).
 
   Definition inBounds :=
     ( LETE inRangeVal <- inRange;
       RetE ((x >= #inRangeVal @% "base") && (ZeroExtend 1 x < #inRangeVal @% "top"))).
 
   Definition systemAccess :=
-    ( LETE perms <- capPerms inCap;
+    ( LETC perms <- getCapPerms inCap;
       RetE (#perms @% "SR") ).
 End InBoundsTy.
 
 Section InBoundsInits.
   Variable x: word 32.
-  Variable rfInit: Fin.t 32 -> type FullCapWithTagKind.
-  Variable capPcInit: word 32.
+  Variable rfInit: Fin.t 32 -> type FullCapWithTag.
+  Variable capPcInit: type Cap.
   Variable valPcInit: word 32.
 
   Local Open Scope kami_expr.
@@ -31,35 +33,36 @@ Section InBoundsInits.
                              (Var type (SyntaxKind _) (rfInit i) @% "cap")
                              (Var type (SyntaxKind _) (rfInit i) @% "val")) = true.
   Definition InBoundsPc :=
-    evalLetExpr (inBounds (Const _ x) (Const _ capPcInit) (Const _ valPcInit)) = true.
+    evalLetExpr (inBounds (Const _ x) (Const _ (convTypeToConst capPcInit)) (Const _ valPcInit)) = true.
 
   Definition SystemAccessRf :=
     exists i, evalLetExpr (systemAccess (Var type (SyntaxKind _) (rfInit i) @% "cap")) = true.
 
   Definition SystemAccessPc :=
-    evalLetExpr (systemAccess (Const _ capPcInit)) = true.
+    evalLetExpr (systemAccess (Const _ (convTypeToConst capPcInit))) = true.
 End InBoundsInits.
 
 Section InBoundsCoreConfig.
   Variable x: word 32.
   Variable p: CoreConfigParams.
-  Definition InBoundsInit := InBoundsRf x (@regsInitVal p) \/ InBoundsPc x (@pcCapInitVal p) (@pcValInitVal p).
-  Definition SystemAccessInit := SystemAccessRf (@regsInitVal p) \/ SystemAccessPc (@pcCapInitVal p).
+  Definition InBoundsInit := InBoundsRf x (@regsInit p) \/ InBoundsPc x (@pcCapInit p)
+                                                             (wcombine (@pcValInit p) (wzero 2)).
+  Definition SystemAccessInit := SystemAccessRf (@regsInit p) \/ SystemAccessPc (@pcCapInit p).
 End InBoundsCoreConfig.
 
 Record SpecIsolation := {
     cores: list CoreConfigParams;
-    disjointNamesCores: NoDup (map (@prefix) cores);
+    disjointNamesCores: NoDup (map (@procName) cores);
     disjointBoundsCores: forall x p, In p cores -> InBoundsInit x p -> forall q,
-                                         In q cores -> InBoundsInit x q -> @prefix p <> @prefix q -> False;
+                                         In q cores -> InBoundsInit x q -> @procName p <> @procName q -> False;
     noScrAccessCores: forall p, In p cores -> SystemAccessInit p -> False;
-    noTrapCores: forall p, In p cores -> @hasTrapVal p = false;
+    noTrapCores: forall p, In p cores -> @hasTrap p = false;
     trapCore: CoreConfigParams;
-    trapCoreMemSize: forall p, In p cores -> @LgNumMemBytesVal p = @LgNumMemBytesVal trapCore;
+    trapCoreMemSize: forall p, In p cores -> @LgNumMemBytes (@memParams p) = @LgNumMemBytes (@memParams trapCore);
     disjointTrapCore: forall x p, In p cores -> InBoundsInit x p -> InBoundsInit x trapCore -> False;
     sameMemTrapCore: forall x p,
       In p cores -> InBoundsInit x p ->
-      evalExpr (Var type (SyntaxKind (Array _ (Bit 8))) (@memInitVal trapCore) @[Const _ x])%kami_expr =
-        evalExpr (Var type (SyntaxKind (Array _ (Bit 8)))(@memInitVal p) @[Const _ x])%kami_expr;
-    trapCoreHasTrap: @hasTrapVal trapCore = true;
+      evalExpr (Var type (SyntaxKind (Array _ (Bit 8))) (@memInit (@memParams trapCore)) @[Const _ x])%kami_expr =
+        evalExpr (Var type (SyntaxKind (Array _ (Bit 8)))(@memInit (@memParams p)) @[Const _ x])%kami_expr;
+    trapCoreHasTrap: @hasTrap trapCore = true;
   }.
